sorting seems to work

src/sort_experiments.lean
@@ -1,14 +1,174 @@
 import data.list.pairwise
+import tactic
 namespace list
+
+variable r : ℕ → ℕ → Prop
+
+
+/-
+The great thing about using the for all formulation rather than comparing against just the list head
+is that the forall formulation automatically handles the case that a one element list is sorted. 
+
+-/
+inductive jtsort : list ℕ → Prop
+| nil : jtsort [] 
+| cons : ∀ (a : ℕ ) (l : list ℕ ), (∀ a' ∈ l, a≥ a') → jtsort l → jtsort (a::l) 
+
+
+lemma jtsort_cons2 (a : ℕ ) (l : list ℕ ) : jtsort (a::l) ↔ (∀ a' ∈ l, a≥ a') ∧ jtsort (l)
+:=
+begin
+  split,
+  intro h,
+  cases h with h1 h2 h3 h4,
+  exact and.intro h3 h4,
+  intro h,
+  cases h with h1 h2 h3 h4,
+  apply jtsort.cons a l h1 h2,
+end
+
+
+/-
+lemma: If l is sorted, and a∈ ℕ, then stinsert a l is also sorted.
+Proof.
+if l is nil, then stinsert a l is [a] which is sorted. 
+
+Otherwise, write l=(b::s). Then stinsert a l depends on whether a≥ b or not.
+if a ≥ b, then stinsert a (b::s) = a::b::s. Since l=(b::s), is sorted, we know that,
+for all b' in l, b≥ b'.  We also know a ≥ b. Therefore a≥ b' for all b' and so (a::b::l) is sorted. 
+
+If a < b, then stinsert a (b::s) is b::(stinsert a s).  Since s is shorter than then l,
+we know by induction that stinsert a s is sorted.  We also know that b ≥ every element of stinsert a s 
+because b is greater then or equal to  every element of s by assumption, and b>a by hypothesis. 
+Therefore b::(stinsert a s) is sorted. 
+-/
+
+
 
 def stinsert  : ℕ → list ℕ → list ℕ 
 | a  [] := [a]
-| a  (b::l) := if a ≥  b then a::b::l else b::(stinsert a l)
+| a  (b::l) := if a ≥ b then a::b::l else b::(stinsert a l)
 
 def srt : list ℕ → list ℕ 
 | [] := []
 | (a::l) := stinsert a (srt l)
 
+#check list ℕ 
+
+#eval srt [1,2,3]
+
+lemma nil_sorted : ∀ (l : list ℕ), (l=[]) → jtsort l
+:=
+begin
+  intro l,
+  cases l with hd tl,
+  intro,
+  exact jtsort.nil,
+  intro h,
+  contradiction,
+end
+
+lemma tail_sorted : ∀ (a : ℕ ) (l : list ℕ ), jtsort (a::l) → jtsort l :=
+begin
+  intros a l H,
+  cases H with a l h1 h2,
+  exact h2,
+end
+
+
+lemma step : ∀ (a b: ℕ ) (l : list ℕ ), (∀ (a'∈ l), (b≥a')) ∧ (a≥ b) → ∀ (a' ∈ (b::l)), a≥ a' :=
+begin
+  intros a b l H,
+  cases H with Ha Hb,
+  intro x,
+  intro Hab,
+  cases Hab,
+  have Hba := eq.symm Hab,
+  subst_vars,
+  exact Hb,
+  have  hK:= Ha x Hab,
+  linarith,
+end
+
+
+
+lemma un : ∀ (a x : ℕ) (l : list ℕ ), (x ∈ (stinsert a l)) → (x ∈ (a::l)) :=
+begin
+  intros a x l,
+  induction l with hd tl H,
+  intro h,
+  cases h,
+  subst h,
+  apply mem_singleton_self,
+  cases h,
+  rw stinsert,
+  split_ifs,
+  intro H,
+  exact H,
+  intro H1,
+  have Hk := eq_or_ne_mem_of_mem H1,
+  cases Hk,
+  subst Hk,
+  simp,
+  cases Hk,
+  have Hn := H Hk_right,
+  by_cases x=a,
+  subst h,
+  simp,
+  have Hm := mem_of_ne_of_mem h Hn,
+  rw mem_cons_iff,
+  right,
+  rw mem_cons_iff,
+  right,
+  exact Hm,
+end
+
+
+
+lemma ins_sorted : ∀ (a : ℕ ) (l : list ℕ ), jtsort l → jtsort (stinsert a l):=
+begin
+  intros a l H,
+  induction l with b l iH,
+  rw stinsert,
+  have hK := (jtsort.cons a []) _ H,
+  exact hK,
+  intros a' hN,
+  cases hN,
+  rw stinsert,
+  split_ifs,
+  cases H with a l H1 H2,
+  have hK := step a b l (and.intro H1 h),
+  have HZ := jtsort.cons b l H1 H2,
+  exact jtsort.cons a (b::l) hK HZ,
+  have HW := tail_sorted b l H,
+  have HN := iH HW,
+  apply jtsort.cons, 
+  intro x,
+  intro Hx,
+  have HM := jtsort_cons2 b l,
+  cases HM with HL HR,
+  have HP1 := (HL H).left,
+  have Hz := un a x l Hx,
+  rw mem_cons_iff at Hz,
+  cases Hz,
+  linarith,
+  exact HP1 x Hz,
+  exact HN,
+end
+
+
+
+theorem jtsorter : ∀ (l : list ℕ ), jtsort (srt l):=
+begin
+  intro,
+  induction l with a l ih,
+  rw srt,
+  apply nil_sorted,
+  refl,
+  rw srt,
+  have HK := ins_sorted a l.srt ih,
+  exact HK,
+end
 
 
 end list
